DependentComputability/Tactic/Computability.lean
@@ -1,0 +1,252 @@
+import DependentComputability.Tactic.NewDPrimStep
+import DependentComputability.Tactic.ConvertToNew
+import DependentComputability.Tactic.Delab
+
+convert_to_new Acc
+
+open scoped Delab
+
+open Nat.Partrec Denumerable in
+private def selfCallWith (x : ℕ) : Part ℕ :=
+  (ofNat Code x.unpair.1).eval x
+
+open Nat.Partrec Denumerable Encodable in
+private def thing (selfCallWith : Code) (x : ℕ) : Part ℕ :=
+  x.unpaired fun f x => x.unpaired fun x n =>
+    (ofNat Code f).eval (Nat.pair n (encode (selfCallWith.curry x)))
+
+open Nat.Partrec Denumerable Encodable in
+private def ycomb (thing : Code) (x : ℕ) : Part ℕ :=
+  x.unpaired fun f n =>
+    (thing.curry f).eval (Nat.pair (encode (thing.curry f)) n)
+
+open Nat.Partrec in
+private theorem selfCallWith_part : Nat.Partrec selfCallWith := by
+  rw [← Partrec.nat_iff]
+  exact Code.eval_part.comp (.comp (.ofNat _) (.comp .fst .unpair)) .id
+
+open Nat.Partrec in
+private theorem thing_part (selfCallWith : Code) : Nat.Partrec (thing selfCallWith) := by
+  rw [← Partrec.nat_iff]
+  refine Code.eval_part.comp (.comp (.ofNat _) (.comp .fst .unpair)) ?_
+  have : Computable₂ Nat.pair := by
+    refine Primrec.to_comp ?_
+    simpa [Primrec] using Nat.Primrec.succ
+  refine this.comp ?_ ?_
+  · exact .comp .snd (.comp .unpair (.comp .snd .unpair))
+  · refine .comp .encode ?_
+    refine Code.primrec₂_curry.to_comp.comp (.const _) ?_
+    exact .comp .fst (.comp .unpair (.comp .snd .unpair))
+
+open Nat.Partrec in
+private theorem ycomb_part (thing : Code) : Nat.Partrec (ycomb thing) := by
+  rw [← Partrec.nat_iff]
+  have : Computable₂ Nat.pair := by
+    refine Primrec.to_comp ?_
+    simpa [Primrec] using Nat.Primrec.succ
+  refine Code.eval_part.comp ?_ ?_
+  · exact Code.primrec₂_curry.to_comp.comp (.const _) (.comp .fst .unpair)
+  · refine this.comp ?_ (.comp .snd .unpair)
+    refine .comp .encode ?_
+    exact Code.primrec₂_curry.to_comp.comp (.const _) (.comp .fst .unpair)
+
+/-open Nat.Partrec (Code) in
+theorem dcomputable_reassoc {α : Sort u} {β : α → Sort v} {γ : (a : α) ×' β a → Sort w}
+    {δ : (x : (a : α) ×' β a) ×' γ x → Sort w'}
+    [EncodingRelation α] [∀ x, EncodingRelation (β x)] [∀ x, EncodingRelation (γ x)]
+    [∀ x, EncodingRelation (δ x)]
+    (f : (x : (x : (a : α) ×' β a) ×' γ x) → δ x) :
+    DComputable f ↔ DComputable fun x : (a : α) ×' (b : β a) ×' γ ⟨a, b⟩ =>
+      f ⟨⟨x.1, x.2.1⟩, x.2.2⟩ := by
+  constructor
+  · intro hf
+    refine DComputable.comp hf (DPrimrec.dcomputable ?_)
+    dprim_tac
+  · intro hf
+    refine DComputable.comp
+      (g := fun x : (x : (a : α) ×' β a) ×' γ x => ⟨x.1.1, x.1.2, x.2⟩) hf ?_
+    refine DPrimrec.dcomputable ?_
+    dprim_tac-/
+
+/-open Nat.Partrec Denumerable in
+theorem New.Acc.rec.computable.{c, v, u}
+    {ctx_base : Sort c}
+    {ctx : convert_to_new_type% ctx_base}
+    {α_base : ctx_base → Sort u}
+    {α : convert_to_new_type% α_base}
+    {r_base : (c : ctx_base) → α_base c → α_base c → Prop}
+    {r : convert_to_new_type% r_base}
+    {motive_base : (c : ctx_base) → (a : α_base c) → _root_.Acc (r_base c) a → Sort v}
+    {motive : convert_to_new_type% motive_base}
+    {intro_base : (c : ctx_base) → (a : α_base c) →
+        (h : ∀ b, r_base c b a → _root_.Acc (r_base c) b) →
+      (ih : ∀ b hb, motive_base c b (h b hb)) → motive_base c a (_root_.Acc.intro a h)}
+    {intro : convert_to_new_type% intro_base}
+    (intro_comp : DComputable (convert_to_new% intro_base))
+    {a_base : (c : ctx_base) → α_base c}
+    {a : convert_to_new_type% a_base}
+    (a_comp : DComputable (convert_to_new% a_base))
+    {t_base : (c : ctx_base) → _root_.Acc (r_base c) (a_base c)}
+    {t : convert_to_new_type% t_base} :
+    DComputable (convert_to_new% fun c => @_root_.Acc.rec
+      (α_base c) (r_base c) (motive_base c) (intro_base c) (a_base c) (t_base c)) := by
+  by_cases hprop : IsProp.{imax (max (max 1 u) (imax (max 1 u) v)) v}
+  · exact .of_isProp @(isProp_of_isProp_imax.{max (max 1 u) (imax (max 1 u) v), v} hprop)
+  by_cases hprop : IsProp.{imax (max 1 u) v}
+  · exact .of_isProp @(isProp_of_isProp_imax.{max 1 u, v} hprop)
+  /-have : DComputable (fun c : ctx =>
+      fun x :
+        (a : { a : α c // ∀ b, r c b a → Acc (r c) b }) ×'
+          (∀ b : { b // r c b a }, motive c b (a.2 b b.2)) =>
+          intro c x.1.1 x.1.2 fun b hb => x.2 ⟨b, hb⟩) := by
+    simp only [dcomputable_curry, dcomputable_reassoc] at hintro ⊢
+    let ty := (c : ctx) ×' (a : { a : α c // ∀ b, r c b a → Acc (r c) b }) ×'
+      (∀ b : { b // r c b a }, motive c b (a.2 b b.2))
+    refine DComputable.comp
+      (g := fun a : ty => ⟨a.1, a.2.1.1, a.2.1.2, fun b hb => a.2.2 ⟨b, hb⟩⟩) hintro ?_
+    dprim_tac-/
+  obtain ⟨gi, hgi, hgi'⟩ := this
+  obtain ⟨ga, hga, hga'⟩ := ha
+  obtain ⟨scw, hscw⟩ := Code.exists_code.mp selfCallWith_part
+  obtain ⟨th, hth⟩ := Code.exists_code.mp (thing_part scw)
+  have hyc := ycomb_part th
+  refine ⟨_, .comp hyc (.pair hgi hga), ?_⟩
+  intro n b hn
+  obtain ⟨na, hna, hna'⟩ := hga' hn
+  obtain ⟨ni, hni, hc⟩ := hgi' hn
+  let c := Denumerable.ofNat Code ni
+  rw [encodes_pi_def] at hc
+  clear hga' hgi' hintro
+  specialize t b
+  have (eq := haeq) a := a b
+  dsimp +instances only
+  rw! [← haeq] at t hna' ⊢
+  simp only [Part.eq_some_iff.mpr hni, Part.map_eq_map, Part.map_some, Part.eq_some_iff.mpr hna,
+    seq_eq_bind_map, Part.bind_eq_bind, Part.bind_some]
+  change ∃ y ∈ _, EncodingRelation.Encodes y (@Acc.rec (α b) (r b) (motive b) (intro b) a t)
+  clear hna haeq
+  induction t generalizing na with | intro a ha ih
+  have hycomb : ∃ g, (∀ n, (ofNat Code g).eval n = ycomb th (Nat.pair ni n)) ∧
+      ycomb th (Nat.pair ni na) = c.eval (Nat.pair na g) := by
+    refine ⟨Encodable.encode (scw.curry (Encodable.encode (th.curry ni))), ?_, ?_⟩
+    · intro n
+      simp [hscw, selfCallWith, ycomb]
+    · simp [ycomb, hth, thing, c]
+  obtain ⟨g, hg, hg'⟩ := hycomb
+  specialize hc (Nat.pair na g)
+    ⟨⟨a, ha⟩, fun q => @Acc.rec (α b) (r b) (motive b) (intro b) q.1 (ha q.1 q.2)⟩
+  specialize hc ⟨by simpa using hna', ?_⟩
+  · simp only [Nat.unpair_pair]
+    rw [encodes_pi_def]
+    intro x ⟨y, hy⟩ h
+    obtain ⟨z, hz, hz'⟩ := ih y hy x h
+    simp only [hg]
+    use z, hz, hz'
+  simpa only [hg', c] using hc-/
+
+example : DComputable (convert_to_new% fun x : Nat => x) := by
+  dcomp_tac
+
+attribute [dprim] New.PSigma.fst.computable New.PSigma.snd.computable New.PSigma.mk.computable
+  New.PSigma.fst.primrec New.PSigma.snd.primrec New.PSigma.mk.primrec
+
+@[dprim]
+theorem New.Unit.unit.computable {ctx_base : Sort u} {ctx : convert_to_new_type% ctx_base} :
+    DComputable (convert_to_new% fun _ : ctx_base => ()) := by
+  refine .const' (x := convert_to_new% ()) ?_
+  exact ⟨0, .zero⟩
+
+example : DComputable (convert_to_new% fun (x : Nat → Nat) y => x y) := by
+  dcomp_tac
+
+example : DComputable (convert_to_new% fun (x : Nat → Nat) y => x (x y)) := by
+  dcomp_tac
+
+example : DComputable (convert_to_new% fun (x : Nat → (_ : Nat) ×' Nat) y => x (x y).2) := by
+  dcomp_tac
+
+@[dprim]
+theorem New.Nat.zero.computable {ctx_base : Sort u} {ctx : convert_to_new_type% ctx_base} :
+    DComputable (convert_to_new% fun _ : ctx_base => _root_.Nat.zero) := by
+  refine .const' (x := convert_to_new% _root_.Nat.zero) ?_
+  refine ⟨0, ?_⟩
+  rfl
+
+@[dprim]
+theorem New.Nat.succ.computable {ctx_base : Sort u} {ctx : convert_to_new_type% ctx_base}
+    {f_base : ctx_base → ℕ} {f : convert_to_new_type% f_base}
+    (f_comp : DComputable (convert_to_new% f_base)) :
+    DComputable (convert_to_new% fun c => _root_.Nat.succ (f_base c)) := by
+  refine .comp ?_ (f := convert_to_new% _root_.Nat.succ) f_comp
+  refine ⟨_root_.Nat.succ, .succ, ?_⟩
+  intro a _ _ rfl
+  exact ⟨a + 1, by simp, by rfl⟩
+
+@[dprim]
+theorem New.Nat.rec.primrec {ctx_base : Sort u} {ctx : convert_to_new_type% ctx_base}
+    {motive_base : ctx_base → ℕ → Sort v} {motive : convert_to_new_type% motive_base}
+    {zero_base : (c : ctx_base) → motive_base c .zero}
+    {zero : convert_to_new_type% zero_base}
+    (zero_comp : DPrimrec (convert_to_new% zero_base))
+    {succ_base : (c : ctx_base) → (n : ℕ) → motive_base c n → motive_base c (.succ n)}
+    {succ : convert_to_new_type% succ_base}
+    (succ_comp : DPrimrec (convert_to_new%
+      fun x : (c : ctx_base) ×' (n : ℕ) ×' motive_base c n => succ_base x.1 x.2.1 x.2.2))
+    {t_base : ctx_base → ℕ} {t : convert_to_new_type% t_base}
+    (t_comp : DPrimrec (convert_to_new% t_base)) :
+    DPrimrec (convert_to_new% fun c =>
+      @_root_.Nat.rec (motive_base c) (zero_base c) (succ_base c) (t_base c)) := by
+  obtain ⟨fz, hfz, hfz'⟩ := zero_comp
+  obtain ⟨fs, hfs, hfs'⟩ := succ_comp
+  obtain ⟨ft, hft, hft'⟩ := t_comp
+  refine ⟨_, .comp (.prec hfz hfs) (.pair .id hft), ?_⟩
+  intro c_base c nc hnc
+  simp only [Nat.unpaired, id_eq, Nat.unpair_pair]
+  specialize hfz' hnc
+  specialize hft' hnc
+  rw [show t_base c_base = ft nc from hft']
+  induction ft nc with
+  | zero => exact hfz'
+  | succ k ih =>
+    specialize @hfs' ⟨c_base, k, _root_.Nat.rec (zero_base c_base) (succ_base c_base) k⟩
+    specialize @hfs' ⟨c, (), Nat.rec (motive c) (zero c) (succ c) ()⟩
+    exact @hfs' (Nat.pair nc (Nat.pair k _))
+      ⟨by simpa using hnc, by simp; rfl, by simpa using ih⟩
+
+convert_to_new Nat.recAux
+
+@[dprim]
+theorem New.Nat.rec.computable {ctx_base : Sort u} {ctx : convert_to_new_type% ctx_base}
+    {motive_base : ctx_base → ℕ → Sort v} {motive : convert_to_new_type% motive_base}
+    {zero_base : (c : ctx_base) → motive_base c .zero}
+    {zero : convert_to_new_type% zero_base}
+    (zero_comp : DComputable (convert_to_new% zero_base))
+    {succ_base : (c : ctx_base) → (n : ℕ) → motive_base c n → motive_base c (.succ n)}
+    {succ : convert_to_new_type% succ_base}
+    (succ_comp : DComputable (convert_to_new% succ_base))
+    {t_base : ctx_base → ℕ} {t : convert_to_new_type% t_base}
+    (t_comp : DComputable (convert_to_new% t_base)) :
+    DComputable (convert_to_new% fun c =>
+      @_root_.Nat.rec (motive_base c) (zero_base c) (succ_base c) (t_base c)) := by
+  have := convert_to_new%
+    show (fun c => @_root_.Nat.rec (fun n => _root_.Unit → motive_base c n) (fun _ => zero_base c)
+          (fun n ih _ => succ_base c n (ih ())) (t_base c) ()) =
+        (fun c => @_root_.Nat.rec (motive_base c) (zero_base c) (succ_base c) (t_base c)) by
+      funext c; induction t_base c <;> simp_all
+  dsimp only at this
+  refine Eq._induct.rec (motive := fun a _ _ => DComputable a) ?_ this
+  dsimp only
+  have recComp : DComputable (convert_to_new% fun x :
+      (c : ctx_base) ×' (zero : _root_.Unit → motive_base c 0) ×'
+        (succ : (n : ℕ) → (_root_.Unit → motive_base c n) →
+          _root_.Unit → motive_base c (n.succ)) ×' ℕ =>
+      @_root_.Nat.rec (fun n => _root_.Unit → motive_base x.1 n) x.2.1 x.2.2.1 x.2.2.2) := by
+    refine .of_prim ?_
+    dcomp_tac
+  have mk : DComputable (convert_to_new% fun c : ctx_base =>
+      (⟨c, fun _ => zero_base c, fun n ih _ => succ_base c n (ih ()), t_base c⟩ :
+        (c : ctx_base) ×' (zero : _root_.Unit → motive_base c 0) ×'
+          (succ : (n : ℕ) → (_root_.Unit → motive_base c n) →
+            _root_.Unit → motive_base c (n.succ)) ×' ℕ)) := by
+    dcomp_tac
+  exact .comp (.app recComp Unit.unit.computable) mk
