DependentComputability/Tactic/Delab.lean
@@ -1,0 +1,63 @@
+import DependentComputability.SortExtra
+
+namespace Delab
+
+open Lean PrettyPrinter Delaborator SubExpr Meta
+
+partial def convertBackFromNew (e : Expr) : OptionT MetaM Expr := do
+  match e with
+  | .lam nm' t_base (.lam nm t b bi) bi' =>
+    withLocalDecl nm' bi' t_base fun var_base => do
+    withLocalDecl nm bi (t.instantiate1 var_base) fun var => do
+      let res ← convertBackFromNew (b.instantiate #[var_base, var])
+      if res.hasAnyFVar (· == var.fvarId!) then failure
+      mkLambdaFVars #[var_base] res
+  | .letE nm' t_base v_base (.letE nm t v b nd) nd' =>
+    withLetDecl nm' t_base v_base fun var_base => do
+    withLetDecl nm (t.instantiate1 var_base) (v.instantiate1 var_base) fun var => do
+      let res ← convertBackFromNew (b.instantiate #[var_base, var])
+      if res.hasAnyFVar (· == var.fvarId!) then failure
+      return .letE nm t_base v_base (res.abstract #[var_base]) nd
+  | .const nm us =>
+    let some nm := (`New).isPrefixOf? nm | failure
+    if nm = `Sort then
+      let [u] := us | failure
+      return .sort u
+    return .const nm us
+  | .app .. =>
+    e.withApp fun fn args => do
+      if ¬2 ∣ args.size then failure
+      if let .const ``New.Forall .. := fn then
+        let #[_α_base, _α, .lam nm t_base b_base bi, _β_base] := args | failure
+        return .forallE nm t_base b_base bi
+      else if let .const `uniqueNatLit .. := fn then
+        let #[n] := args | failure
+        return n
+      else if let .const `uniqueStrLit .. := fn then
+        let #[s] := args | failure
+        return s
+      let mut expr ← convertBackFromNew fn
+      for h : i in *...(args.size/2) do
+        have : i < args.size/2 := h
+        expr := expr.app args[i * 2]
+      return expr
+  | .fvar var =>
+    let mkExtraApp _ e ← var.getType | failure
+    return e
+  | .bvar i => failure
+  | _ => failure
+
+@[scoped delab app]
+def delabNew : Delab := whenNotPPOption getPPExplicit do
+  let e ← getExpr
+  if let mkExtraApp _ e := e then
+    withTheReader SubExpr (fun x => { x with expr := e }) do
+    let stx ← delab
+    `(convert_to_new_type% $stx)
+  else
+    let some res ← (convertBackFromNew e).run | failure
+    withTheReader SubExpr (fun x => { x with expr := res }) do
+      let stx ← delab
+      `(convert_to_new% $stx)
+
+end Delab
